theories/zoo_parabs/pool.v
@@ -1,5 +1,7 @@
 From zoo Require Import
   prelude.
+From zoo.common Require Import
+  countable.
 From zoo.iris.bi Require Import
   big_op.
 From zoo.language Require Import
@@ -22,6 +24,7 @@ From zoo Require Import
   options.
 
 Implicit Types b : bool.
+Implicit Types l : location.
 Implicit Types v t ctx hub task fut waiter pred fn : val.
 Implicit Types empty : emptiness.
 
@@ -63,185 +66,184 @@ Proof.
   solve_inG.
 Qed.
 
-Record common := {
-  common_size : nat ;
-  common_hub : val ;
-}.
-Implicit Types 𝑐𝑜𝑚 : common.
-
-Record t := {
-  t_size : nat ;
-  t_hub : val ;
-  t_domains : val ;
-}.
-Implicit Types 𝑡 : t.
-
-#[local] Coercion t_to_val 𝑡 :=
-  ( #𝑡.(t_size),
-    𝑡.(t_hub),
-    𝑡.(t_domains)
-  )%V.
-#[local] Coercion t_to_common 𝑡 :=
-  {|common_size := 𝑡.(t_size) ;
-    common_hub := 𝑡.(t_hub) ;
-  |}.
-
-#[local] Lemma t_to_val_inj' t 𝑡1 𝑡2 :
-  t = 𝑡1 →
-  t = 𝑡2 →
-  𝑡1 = 𝑡2.
-Proof.
-  destruct 𝑡1, 𝑡2. naive_solver.
-Qed.
-#[local] Instance t_to_val_inj :
-  Inj (=) (=) t_to_val.
-Proof.
-  intros ?*. eapply t_to_val_inj'; done.
-Qed.
-
-Record context := {
-  context_size : nat ;
-  context_hub : val ;
-  context_id : nat ;
-}.
-Implicit Types 𝑐𝑡𝑥 : context.
-
-#[local] Coercion context_to_val 𝑐𝑡𝑥 :=
-  ( #𝑐𝑡𝑥.(context_size),
-    𝑐𝑡𝑥.(context_hub),
-    #𝑐𝑡𝑥.(context_id)
-  )%V.
-#[local] Coercion context_to_common 𝑐𝑡𝑥 :=
-  {|common_size := 𝑐𝑡𝑥.(context_size) ;
-    common_hub := 𝑐𝑡𝑥.(context_hub) ;
-  |}.
-
-#[local] Lemma context_to_val_inj' ctx 𝑐𝑡𝑥1 𝑐𝑡𝑥2 :
-  ctx = 𝑐𝑡𝑥1 →
-  ctx = 𝑐𝑡𝑥2 →
-  𝑐𝑡𝑥1 = 𝑐𝑡𝑥2.
-Proof.
-  destruct 𝑐𝑡𝑥1, 𝑐𝑡𝑥2. naive_solver.
-Qed.
-#[local] Instance context_to_val_inj :
-  Inj (=) (=) context_to_val.
-Proof.
-  intros ?*. eapply context_to_val_inj'; done.
-Qed.
-
-#[local] Definition common_to_t 𝑐𝑜𝑚 domains :=
-  {|t_size := 𝑐𝑜𝑚.(common_size) ;
-    t_hub := 𝑐𝑜𝑚.(common_hub) ;
-    t_domains := domains ;
-  |}.
-#[local] Definition common_to_context 𝑐𝑜𝑚 i :=
-  {|context_size := 𝑐𝑜𝑚.(common_size) ;
-    context_hub := 𝑐𝑜𝑚.(common_hub) ;
-    context_id := i ;
-  |}.
-
 Section pool_G.
   Context `{pool_G : SchedulerG Σ}.
 
   Implicit Types Ψ Χ Ξ : val → iProp Σ.
 
-  #[local] Definition task_model 𝑐𝑜𝑚 task Ψ : iProp Σ :=
-    ∀ i empty,
-    ws_hub_std_owner 𝑐𝑜𝑚.(common_hub) i Nonblocked empty -∗
-    WP task (common_to_context 𝑐𝑜𝑚 i) {{ v,
+  Record metadata := {
+    metadata_size : nat ;
+    metadata_hub : val ;
+    metadata_domains : val ;
+  }.
+  Implicit Types γ : metadata.
+
+  #[local] Instance metadata_eq_dec : EqDecision metadata :=
+    ltac:(solve_decision).
+  #[local] Instance metadata_countable :
+    Countable metadata.
+  Proof.
+    solve_countable.
+  Qed.
+
+  Record context := {
+    context_size : nat ;
+    context_hub : val ;
+    context_id : nat ;
+  }.
+  Implicit Types 𝑐𝑡𝑥 : context.
+
+  #[local] Coercion context_to_val 𝑐𝑡𝑥 :=
+    ( #𝑐𝑡𝑥.(context_size),
+      𝑐𝑡𝑥.(context_hub),
+      #𝑐𝑡𝑥.(context_id)
+    )%V.
+
+  #[local] Lemma context_to_val_inj' ctx 𝑐𝑡𝑥1 𝑐𝑡𝑥2 :
+    ctx = 𝑐𝑡𝑥1 →
+    ctx = 𝑐𝑡𝑥2 →
+    𝑐𝑡𝑥1 = 𝑐𝑡𝑥2.
+  Proof.
+    destruct 𝑐𝑡𝑥1, 𝑐𝑡𝑥2. naive_solver.
+  Qed.
+  #[local] Instance context_to_val_inj :
+    Inj (=) (=) context_to_val.
+  Proof.
+    intros ?*. eapply context_to_val_inj'; done.
+  Qed.
+
+  #[local] Definition context_consistent γ 𝑐𝑡𝑥 :=
+    γ.(metadata_size) = 𝑐𝑡𝑥.(context_size) ∧
+    γ.(metadata_hub) = 𝑐𝑡𝑥.(context_hub).
+  #[local] Instance : CustomIpatFormat "context_consistent" :=
+    "(
+      %H𝑐𝑡𝑥{}_size &
+      %H𝑐𝑡𝑥{}_hub
+    )".
+
+  #[local] Definition task_model γ task Ψ : iProp Σ :=
+    ∀ 𝑐𝑡𝑥 empty,
+    ⌜context_consistent γ 𝑐𝑡𝑥⌝ -∗
+    ws_hub_std_owner γ.(metadata_hub) 𝑐𝑡𝑥.(context_id) Nonblocked empty -∗
+    WP task 𝑐𝑡𝑥 {{ v,
       ∃ empty,
-      ws_hub_std_owner 𝑐𝑜𝑚.(common_hub) i Nonblocked empty ∗
+      ws_hub_std_owner γ.(metadata_hub) 𝑐𝑡𝑥.(context_id) Nonblocked empty ∗
       Ψ v
     }}.
 
-  #[local] Definition inv_inner 𝑐𝑜𝑚 : iProp Σ :=
+  #[local] Definition inv_inner γ : iProp Σ :=
     ∃ tasks,
-    ws_hub_std_model 𝑐𝑜𝑚.(common_hub) tasks ∗
+    ws_hub_std_model γ.(metadata_hub) tasks ∗
     [∗ mset] task ∈ tasks,
-      task_model 𝑐𝑜𝑚 task (λ _, True).
+      task_model γ task (λ _, True).
   #[local] Instance : CustomIpatFormat "inv_inner" :=
     "(
       %tasks &
       >Hhub_model &
       Htasks
     )".
-  #[local] Definition inv' 𝑐𝑜𝑚 : iProp Σ :=
-    ws_hub_std_inv 𝑐𝑜𝑚.(common_hub) (nroot.@"hub") (S 𝑐𝑜𝑚.(common_size)) ∗
-    inv (nroot.@"inv") (inv_inner 𝑐𝑜𝑚).
-  #[local] Instance : CustomIpatFormat "inv'" :=
+  #[local] Definition inv_1 γ : iProp Σ :=
+    inv (nroot.@"inv") (inv_inner γ).
+  #[local] Definition inv_2 γ : iProp Σ :=
+    ws_hub_std_inv γ.(metadata_hub) (nroot.@"hub") (S γ.(metadata_size)) ∗
+    inv_1 γ.
+  #[local] Instance : CustomIpatFormat "inv_2" :=
     "(
-      #Hhub{}_inv &
-      #Hinv{}
+      #Hhub_inv{_{}} &
+      #Hinv{_{}}
     )".
   Definition pool_inv t sz : iProp Σ :=
-    ∃ 𝑡,
-    ⌜t = 𝑡⌝ ∗
-    ⌜sz = 𝑡.(t_size)⌝ ∗
-    inv' 𝑡.
+    ∃ l γ,
+    ⌜t = #l⌝ ∗
+    meta l nroot γ ∗
+    ⌜sz = γ.(metadata_size)⌝ ∗
+    inv_2 γ.
   #[local] Instance : CustomIpatFormat "inv" :=
     "(
-      %𝑡{} &
+      %l{} &
+      %γ{} &
       {%Heq{};->} &
+      #Hmeta{_{}} &
       -> &
-      {#Hinv{};(:inv')}
+      {#Hinv{};(:inv_2)}
     )".
 
   Definition pool_model t : iProp Σ :=
-    ∃ 𝑡 empty doms,
-    ⌜t = 𝑡⌝ ∗
-    inv' 𝑡 ∗
-    ws_hub_std_owner 𝑡.(t_hub) 0 Blocked empty ∗
-    array_model 𝑡.(t_domains) DfracDiscarded doms ∗
+    ∃ l γ empty doms,
+    ⌜t = #l⌝ ∗
+    meta l nroot γ ∗
+    l.[size] ↦□ #γ.(metadata_size) ∗
+    l.[hub] ↦□ γ.(metadata_hub) ∗
+    l.[domains] ↦□ γ.(metadata_domains) ∗
+    inv_2 γ ∗
+    ws_hub_std_owner γ.(metadata_hub) 0 Blocked empty ∗
+    array_model γ.(metadata_domains) DfracDiscarded doms ∗
     [∗ list] dom ∈ doms,
       domain_model dom itype_unit.
   #[local] Instance : CustomIpatFormat "model" :=
     "(
-      %𝑡{} &
+      %l{} &
+      %γ{} &
       %empty{} &
       %doms{} &
       {%Heq{};->} &
-      {#Hinv{};(:inv')} &
+      #Hmeta{_{}} &
+      #Hl{}_size &
+      #Hl{}_hub &
+      #Hl{}_domains &
+      {#Hinv{};(:inv_2)} &
       Hhub{}_owner &
       Hdomains{} &
       Hdoms{}
     )".
 
-  Definition pool_context_inv t ctx : iProp Σ :=
-    ∃ 𝑡 𝑐𝑡𝑥,
-    ⌜t = 𝑡⌝ ∗
-    ⌜ctx = 𝑐𝑡𝑥⌝ ∗
-    ⌜𝑡 = 𝑐𝑡𝑥 :> common⌝.
-  #[local] Instance : CustomIpatFormat "context_inv" :=
-    "(
-      %𝑡{} &
-      %𝑐𝑡𝑥{;_} &
-      {%H𝑡{}_eq;->} &
-      %H𝑐𝑡𝑥{}_eq &
-      %Hcommon{}
-    )".
-
-  Definition pool_context_model ctx : iProp Σ :=
-    ∃ 𝑐𝑡𝑥 empty,
-    ⌜ctx = 𝑐𝑡𝑥⌝ ∗
-    inv' 𝑐𝑡𝑥 ∗
+  #[local] Definition context_1 γ 𝑐𝑡𝑥 : iProp Σ :=
+    ∃ empty,
     ws_hub_std_owner 𝑐𝑡𝑥.(context_hub) 𝑐𝑡𝑥.(context_id) Nonblocked empty.
-  #[local] Instance : CustomIpatFormat "context_model" :=
+  #[local] Instance : CustomIpatFormat "context_1" :=
     "(
-      %𝑐𝑡𝑥{} &
       %empty{} &
-      {%H𝑐𝑡𝑥{}_eq;->} &
-      {#Hinv{};(:inv')} &
       Hhub_owner
     )".
+  #[local] Definition context_2 γ 𝑐𝑡𝑥 : iProp Σ :=
+    ⌜context_consistent γ 𝑐𝑡𝑥⌝ ∗
+    inv_2 γ ∗
+    context_1 γ 𝑐𝑡𝑥.
+  #[local] Instance : CustomIpatFormat "context_2" :=
+    "(
+      (:context_consistent {//}) &
+      {#Hinv_{};(:inv_2)} &
+      { {lazy} H𝑐𝑡𝑥{}
+      ; {lazy} H𝑐𝑡𝑥
+      ; (:context_1 ={})
+      ; (:context_1)
+      }
+    )".
+  Definition pool_context t ctx : iProp Σ :=
+    ∃ l γ 𝑐𝑡𝑥,
+    ⌜t = #l⌝ ∗
+    meta l nroot γ ∗
+    ⌜ctx = 𝑐𝑡𝑥⌝ ∗
+    context_2 γ 𝑐𝑡𝑥.
+  #[local] Instance : CustomIpatFormat "context" :=
+    "(
+      %l{} &
+      %γ{} &
+      %𝑐𝑡𝑥{} &
+      {%Heq{};->} &
+      #Hmeta{_{}} &
+      {%H𝑐𝑡𝑥{}_eq;->} &
+      (:context_2 {//} {/lazy/})
+    )".
 
-  Definition pool_future_inv fut Ψ Ξ :=
+  Definition pool_future_inv t fut Ψ Ξ :=
     ivar_3_inv fut Ψ Ξ (λ fut waiter,
       ∀ ctx v,
-      pool_context_model ctx -∗
+      pool_context t ctx -∗
       ivar_3_result fut v -∗
       WP waiter ctx v {{ res,
         ⌜res = ()%V⌝ ∗
-        pool_context_model ctx
+        pool_context t ctx
       }}
     )%I.
 
@@ -251,12 +253,12 @@ Section pool_G.
   Definition pool_future_result :=
     ivar_3_result.
 
-  #[global] Instance pool_future_proper fut :
+  #[global] Instance pool_future_proper t fut :
     Proper (
       (pointwise_relation _ (≡)) ==>
       (pointwise_relation _ (≡)) ==>
       (≡)
-    ) (pool_future_inv fut).
+    ) (pool_future_inv t fut).
   Proof.
     solve_proper.
   Qed.
@@ -266,13 +268,8 @@ Section pool_G.
   Proof.
     apply _.
   Qed.
-  #[global] Instance pool_context_inv_persistent t ctx :
-    Persistent (pool_context_inv t ctx).
-  Proof.
-    apply _.
-  Qed.
-  #[global] Instance pool_future_inv_persistent fut Ψ Ξ :
-    Persistent (pool_future_inv fut Ψ Ξ).
+  #[global] Instance pool_future_inv_persistent t fut Ψ Ξ :
+    Persistent (pool_future_inv t fut Ψ Ξ).
   Proof.
     apply _.
   Qed.
@@ -287,20 +284,20 @@ Section pool_G.
     pool_inv t sz2 -∗
     ⌜sz1 = sz2⌝.
   Proof.
-    iIntros "(:inv =1) (:inv =2)".
-    erewrite (t_to_val_inj' _ 𝑡1 𝑡2); done.
+    iIntros "(:inv =1) (:inv =2)". simplify.
+    iDestruct (meta_agree with "Hmeta_1 Hmeta_2") as %<-. done.
   Qed.
 
-  Lemma pool_future_consumer_divide {fut Ψ Ξ Χ} Χs :
-    pool_future_inv fut Ψ Ξ -∗
+  Lemma pool_future_consumer_divide {t fut Ψ Ξ Χ} Χs :
+    pool_future_inv t fut Ψ Ξ -∗
     pool_future_consumer fut Χ -∗
     (∀ x, Χ x -∗ [∗ list] Χ ∈ Χs, Χ x) ={⊤}=∗
     [∗ list] Χ ∈ Χs, pool_future_consumer fut Χ.
   Proof.
     apply ivar_3_consumer_divide.
   Qed.
-  Lemma pool_future_consumer_split {fut Ψ Χ Ξ} Χ1 Χ2 :
-    pool_future_inv fut Ψ Ξ -∗
+  Lemma pool_future_consumer_split {t fut Ψ Χ Ξ} Χ1 Χ2 :
+    pool_future_inv t fut Ψ Ξ -∗
     pool_future_consumer fut Χ -∗
     (∀ v, Χ v -∗ Χ1 v ∗ Χ2 v) ={⊤}=∗
       pool_future_consumer fut Χ1 ∗
@@ -317,23 +314,23 @@ Section pool_G.
     apply ivar_3_result_agree.
   Qed.
 
-  Lemma pool_future_inv_result fut Ψ Ξ v :
-    pool_future_inv fut Ψ Ξ -∗
+  Lemma pool_future_inv_result t fut Ψ Ξ v :
+    pool_future_inv t fut Ψ Ξ -∗
     pool_future_result fut v ={⊤}=∗
     ▷ □ Ξ v.
   Proof.
     apply ivar_3_inv_result.
   Qed.
-  Lemma pool_future_inv_result' fut Ψ Ξ v :
+  Lemma pool_future_inv_result' t fut Ψ Ξ v :
     £ 1 -∗
-    pool_future_inv fut Ψ Ξ -∗
+    pool_future_inv t fut Ψ Ξ -∗
     pool_future_result fut v ={⊤}=∗
     □ Ξ v.
   Proof.
     apply ivar_3_inv_result'.
   Qed.
-  Lemma pool_future_inv_result_consumer fut Ψ Ξ v Χ :
-    pool_future_inv fut Ψ Ξ -∗
+  Lemma pool_future_inv_result_consumer t fut Ψ Ξ v Χ :
+    pool_future_inv t fut Ψ Ξ -∗
     pool_future_result fut v -∗
     pool_future_consumer fut Χ ={⊤}=∗
       ▷^2 Χ v ∗
@@ -341,9 +338,9 @@ Section pool_G.
   Proof.
     apply ivar_3_inv_result_consumer.
   Qed.
-  Lemma pool_future_inv_result_consumer' fut Ψ Ξ v Χ :
+  Lemma pool_future_inv_result_consumer' t fut Ψ Ξ v Χ :
     £ 2 -∗
-    pool_future_inv fut Ψ Ξ -∗
+    pool_future_inv t fut Ψ Ξ -∗
     pool_future_result fut v -∗
     pool_future_consumer fut Χ ={⊤}=∗
       Χ v ∗
@@ -352,26 +349,30 @@ Section pool_G.
     apply ivar_3_inv_result_consumer'.
   Qed.
 
-  #[local] Lemma pool_execute_spec 𝑐𝑜𝑚 i empty task Ψ :
+  #[local] Lemma pool_execute_spec γ 𝑐𝑡𝑥 task Ψ :
     {{{
-      ws_hub_std_owner 𝑐𝑜𝑚.(common_hub) i Nonblocked empty ∗
-      task_model 𝑐𝑜𝑚 task Ψ
+      context_2 γ 𝑐𝑡𝑥 ∗
+      task_model γ task Ψ
     }}}
-      pool_execute (common_to_context 𝑐𝑜𝑚 i) task
-    {{{ v empty,
+      pool_execute 𝑐𝑡𝑥 task
+    {{{ v,
       RET v;
-      ws_hub_std_owner 𝑐𝑜𝑚.(common_hub) i Nonblocked empty ∗
+      context_1 γ 𝑐𝑡𝑥 ∗
       Ψ v
     }}}.
   Proof.
-    iSteps.
+    iIntros "%Φ ((:context_2) & Htask) HΦ".
+
+    wp_rec.
+    wp_smart_apply (wp_wand with "(Htask [//] [Hhub_owner])").
+    { rewrite H𝑐𝑡𝑥_hub //. }
+    rewrite H𝑐𝑡𝑥_hub. iStepFrameSteps 3.
   Qed.
 
-  #[local] Lemma pool_worker_spec 𝑐𝑜𝑚 i empty ctx :
-    ctx = common_to_context 𝑐𝑜𝑚 i →
+  #[local] Lemma pool_worker_spec {γ ctx} 𝑐𝑡𝑥 :
+    ctx = 𝑐𝑡𝑥 →
     {{{
-      inv' 𝑐𝑜𝑚 ∗
-      ws_hub_std_owner 𝑐𝑜𝑚.(common_hub) i Nonblocked empty
+      context_2 γ 𝑐𝑡𝑥
     }}}
       pool_worker ctx
     {{{
@@ -379,13 +380,14 @@ Section pool_G.
       True
     }}}.
   Proof.
-    iIntros (->) "%Φ ((:inv') & Hhub_owner) HΦ".
-
-    iLöb as "HLöb" forall (empty).
+    iIntros (->) "%Φ (:context_2 lazy=) HΦ".
+    iLöb as "HLöb".
+    iDestruct "H𝑐𝑡𝑥" as "(:context_1)".
 
     wp_rec. rewrite pool_max_round_noyield pool_max_round_yield.
+    wp_pures. rewrite -H𝑐𝑡𝑥_hub.
 
-    awp_smart_apply (ws_hub_std_pop_steal_spec with "[$Hhub_inv $Hhub_owner]") without "HΦ"; [done | lia.. |].
+    awp_apply (ws_hub_std_pop_steal_spec with "[$Hhub_inv $Hhub_owner]") without "HΦ"; [done | lia.. |].
     iInv "Hinv" as "(:inv_inner)".
     iAaccIntro with "Hhub_model"; first iSteps. iIntros ([task |]) "Hhub_model !>".
 
@@ -393,15 +395,17 @@ Section pool_G.
       iDestruct (big_sepMS_disj_union with "Htasks") as "(Htask & Htasks)".
       rewrite big_sepMS_singleton.
       iSplitR "Htask"; first iSteps.
-      iIntros "{%} %empty (Hhub_owner & _) HΦ".
+      clear empty. iIntros "%empty (Hhub_owner & _) HΦ".
 
-      wp_smart_apply (pool_execute_spec with "[$Hhub_owner $Htask]") as (res empty') "(Hhub_owner & _)".
-      wp_smart_apply ("HLöb" with "Hhub_owner HΦ").
+      wp_smart_apply (pool_execute_spec with "[Hhub_owner $Htask]") as (res) "(H𝑐𝑡𝑥 & _)".
+      { iStep 2. rewrite H𝑐𝑡𝑥_hub. iFrame. }
+      wp_smart_apply ("HLöb" with "H𝑐𝑡𝑥 HΦ").
 
     - iSplitL; first iSteps.
-      iIntros "{%} %empty (Hhub_owner & ->) HΦ".
+      clear empty. iIntros "%empty (Hhub_owner & ->) HΦ".
 
-      wp_smart_apply (ws_hub_std_block_spec with "[$Hhub_inv $Hhub_owner]"); first done.
+      wp_pures. rewrite -H𝑐𝑡𝑥_hub.
+      wp_apply (ws_hub_std_block_spec with "[$Hhub_inv $Hhub_owner]"); first done.
       iSteps.
   Qed.
 
@@ -419,54 +423,64 @@ Section pool_G.
   Proof.
     iIntros "%Hsz %Φ _ HΦ".
 
-    wp_rec. rewrite /pool_context.
+    wp_rec. rewrite /pool__code.pool_context.
+
     wp_smart_apply (ws_hub_std_create_spec with "[//]") as (hub) "(#Hhub_inv & Hhub_model & Hhub_owners)"; first lia.
     rewrite Z2Nat.inj_add // Nat.add_1_r.
-    iDestruct "Hhub_owners" as "(Hhub_owner & Hhub_owners)".
-
-    pose 𝑐𝑜𝑚 := {|
-      common_size := ₊sz ;
-      common_hub := hub ;
-    |}.
-
-    iMod (inv_alloc _ _ (inv_inner 𝑐𝑜𝑚) with "[Hhub_model]") as "#Hinv".
-    { iSteps. rewrite big_sepMS_empty //. }
+    iDestruct (big_sepL_seq_cons_1 with "Hhub_owners") as "(Hhub_owner & Hhub_owners)".
 
     wp_smart_apply (ws_hub_std_block_spec with "[$Hhub_inv $Hhub_owner]") as "Hhub_owner"; first done.
-    wp_smart_apply (array_unsafe_initi_spec_disentangled' (λ _ dom, domain_model dom itype_unit) with "[Hhub_owners]") as (domains doms) "(_ & Hdomains & Hdoms)"; first done.
-    { iApply (big_sepL_impl_strong with "Hhub_owners").
-      { simpl_length. }
-      iIntros "!>" (k i1 i2 (-> & Hi1)%lookup_seq (-> & Hi2)%lookup_seq) "Hhub_owner".
-      wp_smart_apply (domain_spawn_spec itype_unit with "[Hhub_owner]"); last iSteps. iIntros "%tid _".
-      iApply wp_thread_id_mono.
-      wp_smart_apply (pool_worker_spec with "[$Hinv $Hhub_owner]"); [| iSteps..].
-      assert ((⁺k + 1)%Z = S k) as -> by lia.
-      rewrite /context_to_val Z2Nat.id //.
-    }
-    iMod (array_model_persist with "Hdomains") as "#Hdomains".
-    wp_pures.
 
-    pose 𝑡 := {|
-      t_size := ₊sz ;
-      t_hub := hub ;
-      t_domains := domains ;
+    pose γ 𝑑𝑜𝑚𝑠 := {|
+      metadata_size := ₊sz ;
+      metadata_hub := hub ;
+      metadata_domains := 𝑑𝑜𝑚𝑠 ;
     |}.
 
-    iApply "HΦ".
-    iSplitR.
-    all: iExists 𝑡.
-    all: rewrite /t_to_val Z2Nat.id //.
-    all: iSteps.
+    wp_smart_apply (array_unsafe_initi_spec_disentangled_strong'
+      (λ 𝑑𝑜𝑚𝑠, inv_1 (γ 𝑑𝑜𝑚𝑠))
+      (λ _ dom, domain_model dom itype_unit)
+    with "[Hhub_model Hhub_owners]") as (𝑑𝑜𝑚𝑠 doms) "(_ & Hdomains & #Hinv & Hdoms)"; first done.
+    { iSplitL "Hhub_model".
+
+      - iIntros "!> %𝑑𝑜𝑚𝑠".
+        iApply inv_alloc.
+        iFrame. rewrite big_sepMS_empty //.
+
+      - iApply (big_sepL_impl_strong with "Hhub_owners").
+        { simpl_length. }
+        iIntros "!>" (k i1 i2 (-> & Hi1)%lookup_seq (-> & Hi2)%lookup_seq) "Hhub_owner %𝑑𝑜𝑚𝑠 #Hinv".
+
+        wp_smart_apply (domain_spawn_spec itype_unit with "[Hhub_owner]"); last iSteps. iIntros "%tid _".
+        iApply wp_thread_id_mono.
+
+        pose 𝑐𝑡𝑥 := {|
+          context_size := ₊sz ;
+          context_hub := hub ;
+          context_id := S k ;
+        |}.
+        wp_smart_apply (pool_worker_spec 𝑐𝑡𝑥 with "[$Hinv $Hhub_owner]"); [| iSteps..].
+        { rewrite /context_to_val /=. repeat f_equal; lia. }
+    }
+    iMod (array_model_persist with "Hdomains") as "#Hdomains".
+
+    wp_block l as "Hmeta" "(Hl_size & Hl_hub & Hl_domains & _)".
+    iMod (pointsto_persist with "Hl_size") as "#Hl_size".
+    iMod (pointsto_persist with "Hl_hub") as "#Hl_hub".
+    iMod (pointsto_persist with "Hl_domains") as "#Hl_domains".
+
+    iMod (meta_set (γ 𝑑𝑜𝑚𝑠) with "Hmeta") as "#Hmeta"; first done.
+
+    iSteps.
   Qed.
 
   Lemma pool_run_spec Ψ t task :
     {{{
       pool_model t ∗
       ( ∀ ctx,
-        pool_context_inv t ctx -∗
-        pool_context_model ctx -∗
+        pool_context t ctx -∗
         WP task ctx {{ v,
-          pool_context_model ctx ∗
+          pool_context t ctx ∗
           Ψ v
         }}
       )
@@ -480,15 +494,28 @@ Section pool_G.
   Proof.
     iIntros "%Φ ((:model) & Htask) HΦ".
 
-    wp_rec. rewrite /pool_context.
-    wp_smart_apply (ws_hub_std_unblock_spec with "[$Hhub_inv $Hhub_owner]") as "Hhub_owner"; first done.
-    wp_smart_apply (pool_execute_spec _ 0 _ _ Ψ with "[$Hhub_owner Htask]") as (v empty') "(Hhub_owner & HΨ)".
-    { iIntros "{%} %i %empty Hhub_owner".
-      wp_apply (wp_wand with "(Htask [] [Hhub_owner])") as "%v ((:context_model =1) & $)"; [iSteps.. |].
-      apply (inj context_to_val) in H𝑐𝑡𝑥1_eq as <-.
-      iSteps.
+    wp_rec. rewrite /pool__code.pool_context.
+    wp_load.
+    wp_apply (ws_hub_std_unblock_spec with "[$Hhub_inv $Hhub_owner]") as "Hhub_owner"; first done.
+    do 2 wp_load.
+
+    pose 𝑐𝑡𝑥 := {|
+      context_size := γ.(metadata_size) ;
+      context_hub := γ.(metadata_hub) ;
+      context_id := 0 ;
+    |}.
+    wp_smart_apply (pool_execute_spec _ 𝑐𝑡𝑥 _ Ψ with "[$Hhub_owner Htask]") as (v) "{%} ((:context_1 =1) & HΨ)".
+    { iSplit.
+      - iFrame "#" => //.
+      - iIntros "{%} %𝑐𝑡𝑥 %empty (:context_consistent) Hhub_owner".
+        wp_apply (wp_wand with "(Htask [Hhub_owner])") as (v) "((:context =1) & $)".
+        { iStep 5. rewrite H𝑐𝑡𝑥_hub. iFrame. }
+        apply (inj context_to_val) in H𝑐𝑡𝑥1_eq as <-.
+        rewrite H𝑐𝑡𝑥_hub. iSteps.
     }
-    wp_smart_apply (ws_hub_std_block_spec with "[$Hhub_inv $Hhub_owner]") as "Hhub_owner"; first done.
+
+    wp_load.
+    wp_apply (ws_hub_std_block_spec with "[$Hhub_inv $Hhub_owner]") as "Hhub_owner"; first done.
     iSteps.
   Qed.
 
@@ -504,8 +531,9 @@ Section pool_G.
   Proof.
     iIntros "%Φ (:model) HΦ".
 
-    wp_rec.
+    wp_rec. wp_load.
     wp_smart_apply (ws_hub_std_kill_spec with "Hhub_inv") as "_".
+    wp_load.
     wp_smart_apply (array_iter_spec_disentangled' (λ _ _, True)%I with "[$Hdomains Hdoms]"); last iSteps.
     iApply (big_sepL_impl with "Hdoms"). iIntros "!> %i %dom _ Hdom".
     wp_apply (domain_join_spec with "Hdom").
@@ -515,7 +543,7 @@ Section pool_G.
   Lemma pool_size_spec t sz ctx :
     {{{
       pool_inv t sz ∗
-      pool_context_inv t ctx
+      pool_context t ctx
     }}}
       pool_size ctx
     {{{
@@ -523,112 +551,55 @@ Section pool_G.
       True
     }}}.
   Proof.
-    iIntros "%Φ ((:inv =1) & (:context_inv =2)) HΦ". simplify.
-    wp_rec. wp_pures.
-    apply (f_equal common_size) in Hcommon2 as Hsize2. simpl in Hsize2. rewrite -Hsize2.
-    iSteps.
+    iIntros "%Φ ((:inv =1) & (:context =2)) HΦ". simplify.
+    iDestruct (meta_agree with "Hmeta_1 Hmeta_2") as %<-. iClear "Hmeta_2".
+    rewrite H𝑐𝑡𝑥2_size. iSteps.
   Qed.
 
-  Lemma pool_async_silent_spec_inv t ctx task :
+  Lemma pool_async_silent_spec t ctx task :
     {{{
-      pool_context_inv t ctx ∗
-      pool_context_model ctx ∗
+      pool_context t ctx ∗
       ( ∀ ctx,
-        pool_context_inv t ctx -∗
-        pool_context_model ctx -∗
+        pool_context t ctx -∗
         WP task ctx {{ res,
-          pool_context_model ctx
+          pool_context t ctx
         }}
       )
     }}}
       pool_async_silent ctx task
     {{{
       RET ();
-      pool_context_model ctx
+      pool_context t ctx
     }}}.
   Proof.
-    iIntros "%Φ ((:context_inv) & (:context_model) & Htask) HΦ".
-    apply (inj context_to_val) in H𝑐𝑡𝑥_eq as <-.
+    iIntros "%Φ ((:context) & Htask) HΦ".
 
     wp_rec.
+    wp_pures. rewrite -H𝑐𝑡𝑥_hub.
 
-    awp_smart_apply (ws_hub_std_push_spec with "[$Hhub_inv $Hhub_owner]") without "HΦ"; first done.
+    awp_apply (ws_hub_std_push_spec with "[$Hhub_inv $Hhub_owner]") without "HΦ"; first done.
     iInv "Hinv" as "(:inv_inner)".
-    iAaccIntro with "Hhub_model"; first iFrameSteps. iIntros "Hhub_model".
-    iSplitL. { iFrame. rewrite big_sepMS_singleton. iSteps. }
-    iSteps.
-  Qed.
-  Lemma pool_async_silent_spec ctx task :
-    {{{
-      pool_context_model ctx ∗
-      ( ∀ ctx,
-        pool_context_model ctx -∗
-        WP task ctx {{ res,
-          pool_context_model ctx
-        }}
-      )
-    }}}
-      pool_async_silent ctx task
-    {{{
-      RET ();
-      pool_context_model ctx
-    }}}.
-  Proof.
-    iIntros "%Φ ((:context_model) & Htask) HΦ".
-
-    wp_rec.
-
-    awp_smart_apply (ws_hub_std_push_spec with "[$Hhub_inv $Hhub_owner]") without "HΦ"; first done.
-    iInv "Hinv" as "(:inv_inner)".
-    iAaccIntro with "Hhub_model"; first iFrameSteps. iIntros "Hhub_model".
-    iSplitL. { iFrame. rewrite big_sepMS_singleton. iSteps. }
-    iSteps.
-  Qed.
-
-  Lemma pool_async_spec_inv Ψ Ξ t ctx task :
-    {{{
-      pool_context_inv t ctx ∗
-      pool_context_model ctx ∗
-      ( ∀ ctx,
-        pool_context_inv t ctx -∗
-        pool_context_model ctx -∗
-        WP task ctx {{ v,
-          pool_context_model ctx ∗
-          ▷ Ψ v ∗
-          ▷ □ Ξ v
-        }}
-      )
-    }}}
-      pool_async ctx task
-    {{{ fut,
-      RET fut;
-      pool_context_model ctx ∗
-      pool_future_inv fut Ψ Ξ ∗
-      pool_future_consumer fut Ψ
-    }}}.
-  Proof.
-    iIntros "%Φ (Hctx_inv & Hctx_model & Htask) HΦ".
-
-    wp_rec.
-    wp_smart_apply (ivar_3_create_spec Ψ Ξ with "[//]") as (ivar) "(#Hivar_inv & Hivar_producer & Hivar_consumer)".
-    wp_smart_apply (pool_async_silent_spec_inv with "[$Hctx_inv $Hctx_model Htask Hivar_producer]") as "Hctx_model".
-    { iIntros "{%} %ctx Hctx_inv Hctx_model".
-      wp_smart_apply (wp_wand with "(Htask Hctx_inv Hctx_model)") as (v) "(Hctx_model & HΨ & HΞ)".
-      wp_smart_apply (ivar_3_set_spec with "[$Hivar_inv $Hivar_producer $HΨ $HΞ]") as (waiters) "(#Hivar_result & Hwaiters)".
-      wp_smart_apply (lst_iter_spec' (λ _ _, pool_context_model ctx)%I with "[$Hctx_model Hwaiters]") as "$"; try done.
-      iApply (big_sepL_impl with "Hwaiters").
-      iSteps.
+    iAaccIntro with "Hhub_model"; first iFrameSteps. iIntros "Hhub_model !>".
+    iSplitL.
+    { iFrame. rewrite big_sepMS_singleton.
+      iIntros "{%} !> %𝑐𝑡𝑥 %empty (:context_consistent) Hhub_owner".
+      wp_apply (wp_wand with "(Htask [Hhub_owner])") as (res) "(:context =1)".
+      { iStep 5. rewrite H𝑐𝑡𝑥_hub. iFrame. }
+      apply (inj context_to_val) in H𝑐𝑡𝑥1_eq as <-.
+      rewrite H𝑐𝑡𝑥_hub. iSteps.
     }
-    wp_pures.
-    iApply ("HΦ" with "[$]").
+    iIntros "Hhub_owner HΦ".
+
+    iStep 6. rewrite H𝑐𝑡𝑥_hub. iFrame.
   Qed.
-  Lemma pool_async_spec Ψ Ξ ctx task :
+
+  Lemma pool_async_spec Ψ Ξ t ctx task :
     {{{
-      pool_context_model ctx ∗
+      pool_context t ctx ∗
       ( ∀ ctx,
-        pool_context_model ctx -∗
+        pool_context t ctx -∗
         WP task ctx {{ v,
-          pool_context_model ctx ∗
+          pool_context t ctx ∗
           ▷ Ψ v ∗
           ▷ □ Ξ v
         }}
@@ -637,8 +608,8 @@ Section pool_G.
       pool_async ctx task
     {{{ fut,
       RET fut;
-      pool_context_model ctx ∗
-      pool_future_inv fut Ψ Ξ ∗
+      pool_context t ctx ∗
+      pool_future_inv t fut Ψ Ξ ∗
       pool_future_consumer fut Ψ
     }}}.
   Proof.
@@ -646,21 +617,27 @@ Section pool_G.
 
     wp_rec.
     wp_smart_apply (ivar_3_create_spec Ψ Ξ with "[//]") as (ivar) "(#Hivar_inv & Hivar_producer & Hivar_consumer)".
+
     wp_smart_apply (pool_async_silent_spec with "[$Hctx Htask Hivar_producer]") as "Hctx".
-    { iIntros "{%} %ctx Hctx".
+    { clear ctx. iIntros "%ctx Hctx".
+
       wp_smart_apply (wp_wand with "(Htask Hctx)") as (v) "(Hctx & HΨ & HΞ)".
       wp_smart_apply (ivar_3_set_spec with "[$Hivar_inv $Hivar_producer $HΨ $HΞ]") as (waiters) "(#Hivar_result & Hwaiters)".
-      wp_smart_apply (lst_iter_spec' (λ _ _, pool_context_model ctx)%I with "[$Hctx Hwaiters]") as "$"; try done.
+      wp_smart_apply (lst_iter_spec' (λ _ _, pool_context t ctx)%I with "[$Hctx Hwaiters]") as "$"; try done.
+
       iApply (big_sepL_impl with "Hwaiters").
-      iSteps.
+      iIntros "!> %i %waiter %Hwaiters_lookup Hwaiter Hctx".
+      wp_smart_apply (wp_wand with "(Hwaiter [$] [$])") as (res) "(-> & $) //".
     }
+
     wp_pures.
+
     iApply ("HΦ" with "[$]").
   Qed.
 
-  Lemma pool_wait_until_spec P ctx pred :
+  Lemma pool_wait_until_spec P t ctx pred :
     {{{
-      pool_context_model ctx ∗
+      pool_context t ctx ∗
       □ WP pred () {{ res,
         ∃ b,
         ⌜res = #b⌝ ∗
@@ -670,32 +647,40 @@ Section pool_G.
       pool_wait_until ctx pred
     {{{
       RET ();
-      pool_context_model ctx ∗
+      pool_context t ctx ∗
       P
     }}}.
   Proof.
-    iIntros "%Φ ((:context_model) & #Hpred) HΦ".
-
-    iLöb as "HLöb" forall (empty).
+    iIntros "%Φ ((:context lazy=) & #Hpred) HΦ".
+    iLöb as "HLöb".
+    iDestruct "H𝑐𝑡𝑥" as "(:context_1)".
 
     wp_rec. rewrite pool_max_round_noyield.
     wp_smart_apply (wp_wand with "Hpred") as (res) "(%b & -> & HP)".
-    destruct b; first iSteps.
-    awp_smart_apply (ws_hub_std_pop_steal_until_spec P with "[$Hhub_inv $Hhub_owner $Hpred]") without "HΦ"; [lia.. |].
+    destruct b; first iStepFrameSteps 8.
+
+    awp_smart_apply (ws_hub_std_pop_steal_until_spec P with "[$Hhub_owner $Hpred]") without "HΦ".
+    { lia. }
+    { lia. }
+    { rewrite H𝑐𝑡𝑥_hub //. }
     iInv "Hinv" as "(:inv_inner)".
-    iAaccIntro with "Hhub_model"; first iSteps. iIntros ([task |]) "Hhub_model !>"; last iSteps.
+    rewrite -H𝑐𝑡𝑥_hub.
+    iAaccIntro with "Hhub_model"; first iSteps. iIntros ([task |]) "Hhub_model !>"; last first.
+    { iStep 9. iFrame "#∗". rewrite H𝑐𝑡𝑥_hub. iFrameSteps. }
     iDestruct "Hhub_model" as "(%tasks' & -> & Hhub_model)".
     iDestruct (big_sepMS_insert with "Htasks") as "(Htask & Htasks')".
     iSplitR "Htask"; first iSteps.
-    iIntros "{%} %empty (Hhub_owner & _) HΦ".
+    clear empty. iIntros "%empty (Hhub_owner & _) HΦ".
 
-    wp_smart_apply (pool_execute_spec with "[$Hhub_owner $Htask]") as (res empty') "(Hhub_owner & _)".
-    wp_smart_apply ("HLöb" with "Hhub_owner HΦ").
+    wp_smart_apply (pool_execute_spec with "[Hhub_owner $Htask]") as (res) "(H𝑐𝑡𝑥 & _)".
+    { iStep 2. rewrite H𝑐𝑡𝑥_hub. iFrame. }
+
+    wp_smart_apply ("HLöb" with "H𝑐𝑡𝑥 HΦ").
   Qed.
 
-  Lemma pool_wait_while_spec P ctx pred :
+  Lemma pool_wait_while_spec P t ctx pred :
     {{{
-      pool_context_model ctx ∗
+      pool_context t ctx ∗
       □ WP pred () {{ res,
         ∃ b,
         ⌜res = #b⌝ ∗
@@ -705,7 +690,7 @@ Section pool_G.
       pool_wait_while ctx pred
     {{{
       RET ();
-      pool_context_model ctx ∗
+      pool_context t ctx ∗
       P
     }}}.
   Proof.
@@ -717,16 +702,16 @@ Section pool_G.
     destruct b; iSteps.
   Qed.
 
-  Lemma pool_wait_spec ctx fut Ψ Ξ :
+  Lemma pool_wait_spec t ctx fut Ψ Ξ :
     {{{
-      pool_context_model ctx ∗
-      pool_future_inv fut Ψ Ξ
+      pool_context t ctx ∗
+      pool_future_inv t fut Ψ Ξ
     }}}
       pool_wait ctx fut
     {{{ v,
       RET v;
       £ 2 ∗
-      pool_context_model ctx ∗
+      pool_context t ctx ∗
       pool_future_result fut v
     }}}.
   Proof.
@@ -742,23 +727,23 @@ Section pool_G.
     iApply ("HΦ" with "[$]").
   Qed.
 
-  Lemma pool_iter_spec ctx fut Ψ Ξ fn :
+  Lemma pool_iter_spec t ctx fut Ψ Ξ fn :
     {{{
-      pool_context_model ctx ∗
-      pool_future_inv fut Ψ Ξ ∗
+      pool_context t ctx ∗
+      pool_future_inv t fut Ψ Ξ ∗
       ( ∀ ctx v,
-        pool_context_model ctx -∗
+        pool_context t ctx -∗
         pool_future_result fut v -∗
         WP fn ctx v {{ res,
           ⌜res = ()%V⌝ ∗
-          pool_context_model ctx
+          pool_context t ctx
         }}
       )
     }}}
       pool_iter ctx fut fn
     {{{
       RET ();
-      pool_context_model ctx
+      pool_context t ctx
     }}}.
   Proof.
     iIntros "%Φ (Hctx & #Hivar_inv & Hfn) HΦ".
@@ -768,21 +753,21 @@ Section pool_G.
     all: wp_pures.
 
     - iDestruct "H" as "(_ & #Hivar_result & Hfn)".
-      wp_apply (wp_wand with "(Hfn Hctx Hivar_result)").
-      iSteps.
+      wp_apply (wp_wand with "(Hfn Hctx Hivar_result)") as (res) "(-> & Hctx)".
+      iApply ("HΦ" with "Hctx").
 
     - iApply ("HΦ" with "Hctx").
   Qed.
 
-  Lemma pool_map_spec {ctx fut1 Ψ1 Ξ1} Ψ2 Ξ2 fn :
+  Lemma pool_map_spec {t ctx fut1 Ψ1 Ξ1} Ψ2 Ξ2 fn :
     {{{
-      pool_context_model ctx ∗
-      pool_future_inv fut1 Ψ1 Ξ1 ∗
+      pool_context t ctx ∗
+      pool_future_inv t fut1 Ψ1 Ξ1 ∗
       ( ∀ ctx v1,
-        pool_context_model ctx -∗
+        pool_context t ctx -∗
         pool_future_result fut1 v1 -∗
         WP fn ctx v1 {{ v2,
-          pool_context_model ctx ∗
+          pool_context t ctx ∗
           ▷ Ψ2 v2 ∗
           ▷ □ Ξ2 v2
         }}
@@ -791,8 +776,8 @@ Section pool_G.
       pool_map ctx fut1 fn
     {{{ fut2,
       RET fut2;
-      pool_context_model ctx ∗
-      pool_future_inv fut2 Ψ2 Ξ2 ∗
+      pool_context t ctx ∗
+      pool_future_inv t fut2 Ψ2 Ξ2 ∗
       pool_future_consumer fut2 Ψ2
     }}}.
   Proof.
@@ -800,13 +785,20 @@ Section pool_G.
 
     wp_rec.
     wp_smart_apply (ivar_3_create_spec Ψ2 Ξ2 with "[//]") as (fut2) "(#Hivar2_inv & Hivar2_producer & Hivar2_consumer)".
-    wp_smart_apply (pool_iter_spec with "[$Hctx $Hfut1_inv Hfn Hivar2_producer]"); last iSteps.
-    iIntros "{%} %ctx %v1 Hctx #Hfut1_result".
-    wp_smart_apply (wp_wand with "(Hfn Hctx Hfut1_result)") as (v2) "(Hctx & HΨ2 & HΞ2)".
-    wp_smart_apply (ivar_3_set_spec with "[$Hivar2_inv $Hivar2_producer $HΨ2 $HΞ2]") as (waiters) "(#Hivar2_result & Hwaiters)".
-    wp_smart_apply (lst_iter_spec' (λ _ _, pool_context_model ctx)%I with "[$Hctx Hwaiters]") as "$"; try done.
-    iApply (big_sepL_impl with "Hwaiters").
-    iSteps.
+
+    wp_smart_apply (pool_iter_spec with "[$Hctx $Hfut1_inv Hfn Hivar2_producer]") as "Hctx".
+    { clear ctx. iIntros "%ctx %v1 Hctx #Hfut1_result".
+      wp_smart_apply (wp_wand with "(Hfn Hctx Hfut1_result)") as (v2) "(Hctx & HΨ2 & HΞ2)".
+      wp_smart_apply (ivar_3_set_spec with "[$Hivar2_inv $Hivar2_producer $HΨ2 $HΞ2]") as (waiters) "(#Hivar2_result & Hwaiters)".
+      wp_smart_apply (lst_iter_spec' (λ _ _, pool_context t ctx)%I with "[$Hctx Hwaiters]") as "$"; try done.
+      iApply (big_sepL_impl with "Hwaiters").
+      iIntros "!> %i %waiter %Hwaiters_lookup Hwaiter Hctx".
+      wp_smart_apply (wp_wand with "(Hwaiter [$] [$])") as (res) "(-> & $) //".
+    }
+
+    wp_pures.
+
+    iApply ("HΦ" with "[$]").
   Qed.
 End pool_G.
 
@@ -815,8 +807,7 @@ From zoo_parabs Require
 
 #[global] Opaque pool_inv.
 #[global] Opaque pool_model.
-#[global] Opaque pool_context_inv.
-#[global] Opaque pool_context_model.
+#[global] Opaque pool_context.
 #[global] Opaque pool_future_inv.
 #[global] Opaque pool_future_consumer.
 #[global] Opaque pool_future_result.
