theories/zoo_parabs/pool__code.v
@@ -56,21 +56,21 @@ Definition pool_create : val :=
            domain_spawn
              (fun: <> => pool_worker (pool_context "sz" "hub" ("i" + #1))))
     in
-    ("sz", "hub", "domains").
+    { "sz", "hub", "domains", () }.
 
 Definition pool_run : val :=
   fun: "t" "job" =>
-    ws_hub_std_unblock "t".<hub> #0 ;;
+    ws_hub_std_unblock "t".{hub} #0 ;;
     let: "res" :=
-      pool_execute (pool_context "t".<size> "t".<hub> #0) "job"
+      pool_execute (pool_context "t".{size} "t".{hub} #0) "job"
     in
-    ws_hub_std_block "t".<hub> #0 ;;
+    ws_hub_std_block "t".{hub} #0 ;;
     "res".
 
 Definition pool_kill : val :=
   fun: "t" =>
-    ws_hub_std_kill "t".<hub> ;;
-    array_iter domain_join "t".<domains>.
+    ws_hub_std_kill "t".{hub} ;;
+    array_iter domain_join "t".{domains}.
 
 Definition pool_size : val :=
   fun: "ctx" =>
